% Equation 1
\begin{dmath}
{U}_{t}=\frac{\left({C}_{t}-{{\kappa}}\, {H}_{t}^{{{\theta}}}\, {{\Xi}}_{t}\right)^{1-{{\sigma_{es}}}}-1}{1-{{\sigma_{es}}}}
\end{dmath}
% Equation 2
\begin{dmath}
{{\Xi}}_{t}={C}_{t}^{{{\gamma}}}\, {{\Xi}}_{t-1}^{1-{{\gamma}}}
\end{dmath}
% Equation 3
\begin{dmath}
{UC}_{t}=\left({C}_{t}-{{\kappa}}\, {H}_{t}^{{{\theta}}}\, {{\Xi}}_{t}\right)^{\left(-{{\sigma_{es}}}\right)}
\end{dmath}
% Equation 4
\begin{dmath}
{UL}_{t}={UC}_{t}\, {{\Xi}}_{t}\, {{\kappa}}\, \left(-{{\theta}}\right)\, {H}_{t}^{{{\theta}}-1}
\end{dmath}
% Equation 5
\begin{dmath}
{{\Lambda^{\Xi}}}_{t}={UC}_{t}\, {H}_{t}^{{{\theta}}}\, \left(-{{\kappa}}\right)
\end{dmath}
% Equation 6
\begin{dmath}
{{\lambda}}_{t}={{\beta}}\, {R}_{t}\, {{\lambda}}_{t+1}
\end{dmath}
% Equation 7
\begin{dmath}
{{\lambda}}_{t}={UC}_{t}-\frac{{{\Xi}}_{t}\, {{\gamma}}\, {{\mu}}_{t}}{{C}_{t}}
\end{dmath}
% Equation 8
\begin{dmath}
{{\mu}}_{t}=\frac{\left(1-{{\gamma}}\right)\, {{\beta}}\, {{\mu}}_{t+1}\, {{\Xi}}_{t+1}}{{{\Xi}}_{t}}-{{\Lambda^{\Xi}}}_{t}
\end{dmath}
% Equation 9
\begin{dmath}
\frac{\left(-{UL}_{t}\right)}{{{\lambda}}_{t}}={W}_{t}
\end{dmath}
% Equation 10
\begin{dmath}
{Y}_{t}=\left({H}_{t}\, {A}_{t}\right)^{{{\alpha}}}\, {K}_{t-1}^{1-{{\alpha}}}
\end{dmath}
% Equation 11
\begin{dmath}
\frac{{Y}_{t}\, {{\alpha}}}{{H}_{t}}={W}_{t}
\end{dmath}
% Equation 12
\begin{dmath}
{Y}_{t}={C}_{t}+{G}_{t}+{I}_{t}
\end{dmath}
% Equation 13
\begin{dmath}
{K}_{t}={I}_{t}\, \left(1-{{\phi^X}}\, \left({X}_{t}-1\right)^{2}\right)+{K}_{t-1}\, \left(1-{{\delta}}\right)
\end{dmath}
% Equation 14
\begin{dmath}
{X}_{t}=\frac{{I}_{t}}{{I}_{t-1}}
\end{dmath}
% Equation 15
\begin{dmath}
{\lambda}_{t}=\frac{{UC}_{t}\, {{\beta}}}{{UC}_{t-1}}
\end{dmath}
% Equation 16
\begin{dmath}
{Q}_{t}\, \left(1-{{\phi^X}}\, \left({X}_{t}-1\right)^{2}-\left({X}_{t}-1\right)\, {{\phi^X}}\, 2\, {X}_{t}\right)+2\, {{\phi^X}}\, \left({X}_{t+1}-1\right)\, {X}_{t+1}^{2}\, {Q}_{t+1}\, {\lambda}_{t+1}=1
\end{dmath}
% Equation 17
\begin{dmath}
{R^{K}}_{t}=\frac{\frac{{Y}_{t}\, \left(1-{{\alpha}}\right)}{{K}_{t-1}}+\left(1-{{\delta}}\right)\, {Q}_{t}}{{Q}_{t-1}}
\end{dmath}
% Equation 18
\begin{dmath}
{\lambda}_{t+1}\, {R^{K}}_{t+1}={R}_{t}\, {\lambda}_{t+1}
\end{dmath}
% Equation 19
\begin{dmath}
{G}_{t}={H}_{t}\, {W}_{t}\, {T}_{t}
\end{dmath}
% Equation 20
\begin{dmath}
\log\left({A}_{t}\right)-\log\left((\bar{A})\right)={{\rho_{A}}}\, \left(\log\left({A}_{t-1}\right)-\log\left((\bar{A})\right)\right)+{{\sigma}}\, {epsA}_{t}
\end{dmath}
% Equation 21
\begin{dmath}
\log\left({G}_{t}\right)-\log\left((\bar{G})\right)={{\rho_{G}}}\, \left(\log\left({G}_{t-1}\right)-\log\left((\bar{G})\right)\right)+{{\sigma}}\, {epsG}_{t}
\end{dmath}
% Equation 22
\begin{dmath}
{YY}_{t}=\frac{{Y}_{t}}{(\bar{Y})}
\end{dmath}
% Equation 23
\begin{dmath}
{KK}_{t}=\frac{{K}_{t}}{(\bar{K})}
\end{dmath}
% Equation 24
\begin{dmath}
{II}_{t}=\frac{{I}_{t}}{(\bar{I})}
\end{dmath}
% Equation 25
\begin{dmath}
{CC}_{t}=\frac{{C}_{t}}{(\bar{C})}
\end{dmath}
% Equation 26
\begin{dmath}
{WW}_{t}=\frac{{W}_{t}}{(\bar{W})}
\end{dmath}
% Equation 27
\begin{dmath}
{HH}_{t}=\frac{{H}_{t}}{(\bar{H})}
\end{dmath}
% Equation 28
\begin{dmath}
{RR}_{t}=\frac{{R}_{t}}{(\bar{R})}
\end{dmath}
% Equation 29
\begin{dmath}
{\frac{\bar{K}}{\bar{Y}}}_{t}=\frac{{K}_{t}}{{Y}_{t}}
\end{dmath}
% Equation 30
\begin{dmath}
{\frac{\bar{I}}{\bar{Y}}}_{t}=\frac{{I}_{t}}{{Y}_{t}}
\end{dmath}
% Equation 31
\begin{dmath}
{\frac{\bar{C}}{\bar{Y}}}_{t}=\frac{{C}_{t}}{{Y}_{t}}
\end{dmath}
