% Equation 1
\begin{dmath}
{{\varrho}}_{t}=(\bar{{\varrho}})
\end{dmath}
% Equation 2
\begin{dmath}
{U}_{t}=\frac{\left(\left({C}_{t}-{{\chi}}\, {C}_{t-1}\right)^{1-{{\varrho}}_{t}}\, \left(1-{H}_{t}\right)^{{{\varrho}}_{t}}\right)^{1-{{\sigma_{C}}}}-1}{1-{{\sigma_{C}}}}
\end{dmath}
% Equation 3
\begin{dmath}
{UC}_{t}=\left(1-{{\varrho}}_{t}\right)\, \left({C}_{t}-{{\chi}}\, {C}_{t-1}\right)^{\left(1-{{\varrho}}_{t}\right)\, \left(1-{{\sigma_{C}}}\right)-1}\, \left(1-{H}_{t}\right)^{{{\varrho}}_{t}\, \left(1-{{\sigma_{C}}}\right)}
\end{dmath}
% Equation 4
\begin{dmath}
{UH}_{t}=\left(-{{\varrho}}_{t}\right)\, \left({C}_{t}-{{\chi}}\, {C}_{t-1}\right)^{\left(1-{{\varrho}}_{t}\right)\, \left(1-{{\sigma_{C}}}\right)}\, \left(1-{H}_{t}\right)^{{{\varrho}}_{t}\, \left(1-{{\sigma_{C}}}\right)-1}
\end{dmath}
% Equation 5
\begin{dmath}
{\lambda}_{t}=\frac{{UC}_{t}\, {{\beta}}}{{UC}_{t-1}}
\end{dmath}
% Equation 6
\begin{dmath}
{R}_{t+1}\, {\lambda}_{t+1}=1
\end{dmath}
% Equation 7
\begin{dmath}
{R}_{t}=\frac{{Rn}_{t-1}}{{\pi}_{t}}
\end{dmath}
% Equation 8
\begin{dmath}
{E(R)}_{t}=\frac{{Rn}_{t}}{{\pi}_{t+1}}
\end{dmath}
% Equation 9
\begin{dmath}
\frac{\left(-{UH}_{t}\right)}{{UC}_{t}}={W}_{t}
\end{dmath}
% Equation 10
\begin{dmath}
{\delta}_{t}={{\xi}}\, {\tilde{\pi}}_{t}^{{{\zeta}}}\, {\delta}_{t-1}+\left(1-{{\xi}}\right)\, \left(\frac{{J}_{t}}{{JJ}_{t}}\right)^{\left(-{{\zeta}}\right)}
\end{dmath}
% Equation 11
\begin{dmath}
{Y}_{t}=\frac{\left({H}_{t}\, {A}_{t}\right)^{{{\alpha}}}\, {K}_{t-1}^{1-{{\alpha}}}}{{\delta}_{t}}
\end{dmath}
% Equation 12
\begin{dmath}
{R^{K}}_{t}=\frac{\frac{{\delta}_{t}\, {Y}_{t}\, \left(1-{{\alpha}}\right)\, {P^{W}}_{t}}{{K}_{t-1}}+\left(1-{{\delta}}\right)\, {Q}_{t}}{{Q}_{t-1}}
\end{dmath}
% Equation 13
\begin{dmath}
{Q}_{t}\, \left(1-{S}_{t}-{X}_{t}\, {S^{l}}_{t}\right)+{\lambda}_{t+1}\, {Q}_{t+1}\, {S^{l}}_{t+1}\, {X}_{t+1}^{2}=1
\end{dmath}
% Equation 14
\begin{dmath}
{\lambda}_{t+1}\, {R^{K}}_{t+1}=1
\end{dmath}
% Equation 15
\begin{dmath}
\frac{{P^{W}}_{t}\, {\delta}_{t}\, {Y}_{t}\, {{\alpha}}}{{H}_{t}}={W}_{t}
\end{dmath}
% Equation 16
\begin{dmath}
{Y}_{t}={C}_{t}+{G}_{t}+{I}_{t}
\end{dmath}
% Equation 17
\begin{dmath}
{K}_{t}=\left(1-{S}_{t}\right)\, {I}_{t}+{K}_{t-1}\, \left(1-{{\delta}}\right)
\end{dmath}
% Equation 18
\begin{dmath}
{X}_{t}=\frac{{I}_{t}}{{I}_{t-1}}
\end{dmath}
% Equation 19
\begin{dmath}
{S}_{t}={{\phi_{X}}}\, \left({X}_{t}-1\right)^{2}
\end{dmath}
% Equation 20
\begin{dmath}
{S^{l}}_{t}=\left({X}_{t}-1\right)\, 2\, {{\phi_{X}}}
\end{dmath}
% Equation 21
\begin{dmath}
{G}_{t}={Tax}_{t}
\end{dmath}
% Equation 22
\begin{dmath}
{JJ}_{t}-{{\beta}}\, {{\xi}}\, {\tilde{JJ}}_{t+1}={UC}_{t}\, {Y}_{t}
\end{dmath}
% Equation 23
\begin{dmath}
{J}_{t}-{{\beta}}\, {{\xi}}\, {\tilde{J}}_{t+1}={UC}_{t}\, {Y}_{t}\, \frac{1}{1-\frac{1}{{{\zeta}}}}\, {MC}_{t}\, {MS}_{t}
\end{dmath}
% Equation 24
\begin{dmath}
{\tilde{JJ}}_{t}={JJ}_{t}\, {\tilde{\pi}}_{t}^{{{\zeta}}-1}
\end{dmath}
% Equation 25
\begin{dmath}
{\tilde{J}}_{t}={\tilde{\pi}}_{t}^{{{\zeta}}}\, {J}_{t}
\end{dmath}
% Equation 26
\begin{dmath}
1={{\xi}}\, {\tilde{\pi}}_{t}^{{{\zeta}}-1}+\left(1-{{\xi}}\right)\, \left(\frac{{J}_{t}}{{JJ}_{t}}\right)^{1-{{\zeta}}}
\end{dmath}
% Equation 27
\begin{dmath}
{\tilde{\pi}}_{t}=\frac{{\pi}_{t}}{{\pi}_{t-1}^{{{\gamma^{p}}}}}
\end{dmath}
% Equation 28
\begin{dmath}
\log\left(\frac{{Rn}_{t}}{(\bar{Rn})}\right)={{\rho_{R}}}\, \log\left(\frac{{Rn}_{t-1}}{(\bar{Rn})}\right)+\left(1-{{\rho_{R}}}\right)\, {\theta^{\pi}}\, \log\left(\frac{{\pi}_{t}}{(\bar{\pi})}\right)+\left(1-{{\rho_{R}}}\right)\, {\theta^{y}}\, \log\left(\frac{{Y}_{t}}{(\bar{Y})}\right)+{{\sigma_{M}}}\, {{\epsilon^{M}}}_{t}
\end{dmath}
% Equation 29
\begin{dmath}
{MC}_{t}={P^{W}}_{t}
\end{dmath}
% Equation 30
\begin{dmath}
\log\left({A}_{t}\right)-\log\left((\bar{A})\right)={{\rho_{A}}}\, \left(\log\left({A}_{t-1}\right)-\log\left((\bar{A})\right)\right)+{{\sigma_{A}}}\, {{\epsilon^{A}}}_{t}
\end{dmath}
% Equation 31
\begin{dmath}
\log\left({G}_{t}\right)-\log\left((\bar{G})\right)={{\rho_{G}}}\, \left(\log\left({G}_{t-1}\right)-\log\left((\bar{G})\right)\right)+{{\sigma_{G}}}\, {{\epsilon^{G}}}_{t}
\end{dmath}
% Equation 32
\begin{dmath}
\log\left({GF}_{t}\right)-\log\left((\bar{GF})\right)={{\sigma_{G}}}\, {{\epsilon^{G}}}_{t}+{{\rho_{G}}}\, \left(\log\left({GF}_{t-1}\right)-\log\left((\bar{GF})\right)\right)
\end{dmath}
% Equation 33
\begin{dmath}
\log\left({MS}_{t}\right)-\log\left((\bar{MS})\right)={{\rho_{MS}}}\, \left(\log\left({MS}_{t-1}\right)-\log\left((\bar{MS})\right)\right)+{{\sigma_{MS}}}\, {{\epsilon^{MS}}}_{t}
\end{dmath}
% Equation 34
\begin{dmath}
{yy}_{t}=\frac{{Y}_{t}}{(\bar{Y})}
\end{dmath}
% Equation 35
\begin{dmath}
{kk}_{t}=\frac{{K}_{t}}{(\bar{K})}
\end{dmath}
% Equation 36
\begin{dmath}
{ii}_{t}=\frac{{I}_{t}}{(\bar{I})}
\end{dmath}
% Equation 37
\begin{dmath}
{cc}_{t}=\frac{{C}_{t}}{(\bar{C})}
\end{dmath}
% Equation 38
\begin{dmath}
{ww}_{t}=\frac{{W}_{t}}{(\bar{W})}
\end{dmath}
% Equation 39
\begin{dmath}
{hh}_{t}=\frac{{H}_{t}}{(\bar{H})}
\end{dmath}
% Equation 40
\begin{dmath}
{qq}_{t}=\frac{{Q}_{t}}{(\bar{Q})}
\end{dmath}
% Equation 41
\begin{dmath}
{RR}_{t}=\frac{{R}_{t}}{(\bar{R})}
\end{dmath}
% Equation 42
\begin{dmath}
{E(RR)}_{t}=\frac{{E(R)}_{t}}{(\bar{E(R)})}
\end{dmath}
% Equation 43
\begin{dmath}
{RRn}_{t}=\frac{{Rn}_{t}}{(\bar{Rn})}
\end{dmath}
% Equation 44
\begin{dmath}
{\pi\pi}_{t}=\frac{{\pi}_{t}}{(\bar{\pi})}
\end{dmath}
% Equation 45
\begin{dmath}
{Ogapogap}_{t}=\frac{{OUTGAP}_{t}}{(\bar{OUTGAP})}
\end{dmath}
% Equation 46
\begin{dmath}
{\frac{\bar{K}}{\bar{YW}}}_{t}=\frac{{K}_{t}}{{Y}_{t}}
\end{dmath}
% Equation 47
\begin{dmath}
{\frac{\bar{I}}{\bar{Y}}}_{t}=\frac{{I}_{t}}{{Y}_{t}}
\end{dmath}
% Equation 48
\begin{dmath}
{\frac{\bar{C}}{\bar{Y}}}_{t}=\frac{{C}_{t}}{{Y}_{t}}
\end{dmath}
% Equation 49
\begin{dmath}
{UF}_{t}=\frac{\left(\left({CF}_{t}-{{\chi}}\, {CF}_{t-1}\right)^{1-{{\varrho}}_{t}}\, \left(1-{HF}_{t}\right)^{{{\varrho}}_{t}}\right)^{1-{{\sigma_{C}}}}-1}{1-{{\sigma_{C}}}}
\end{dmath}
% Equation 50
\begin{dmath}
{UCF}_{t}=\left(1-{{\varrho}}_{t}\right)\, \left({CF}_{t}-{{\chi}}\, {CF}_{t-1}\right)^{\left(1-{{\varrho}}_{t}\right)\, \left(1-{{\sigma_{C}}}\right)-1}\, \left(1-{HF}_{t}\right)^{{{\varrho}}_{t}\, \left(1-{{\sigma_{C}}}\right)}
\end{dmath}
% Equation 51
\begin{dmath}
{ULF}_{t}=\left(-{{\varrho}}_{t}\right)\, \left({CF}_{t}-{{\chi}}\, {CF}_{t-1}\right)^{\left(1-{{\varrho}}_{t}\right)\, \left(1-{{\sigma_{C}}}\right)}\, \left(1-{HF}_{t}\right)^{{{\varrho}}_{t}\, \left(1-{{\sigma_{C}}}\right)-1}
\end{dmath}
% Equation 52
\begin{dmath}
{\lambda}_{t}=\frac{{{\beta}}\, {UCF}_{t}}{{UCF}_{t-1}}
\end{dmath}
% Equation 53
\begin{dmath}
{RF}_{t}\, {\lambda}_{t+1}=1
\end{dmath}
% Equation 54
\begin{dmath}
\frac{\left(-{ULF}_{t}\right)}{{UCF}_{t}}={WF}_{t}
\end{dmath}
% Equation 55
\begin{dmath}
{YF}_{t}=\left({A}_{t}\, {HF}_{t}\right)^{{{\alpha}}}\, {KF}_{t-1}^{1-{{\alpha}}}
\end{dmath}
% Equation 56
\begin{dmath}
{RFk}_{t}=\frac{\frac{{YF}_{t}\, \left(1-{{\alpha}}\right)\, {PF^{W}}_{t}}{{KF}_{t-1}}+\left(1-{{\delta}}\right)\, {QF}_{t}}{{QF}_{t-1}}
\end{dmath}
% Equation 57
\begin{dmath}
{QF}_{t}\, \left(1-{SF}_{t}-{XF}_{t}\, {SF^{l}}_{t}\right)+{\lambda}_{t+1}\, {QF}_{t+1}\, {SF^{l}}_{t+1}\, {XF}_{t+1}^{2}=1
\end{dmath}
% Equation 58
\begin{dmath}
{\lambda}_{t+1}\, {RFk}_{t+1}=1
\end{dmath}
% Equation 59
\begin{dmath}
\frac{{PF^{W}}_{t}\, {{\alpha}}\, {YF}_{t}}{{HF}_{t}}={WF}_{t}
\end{dmath}
% Equation 60
\begin{dmath}
{YF}_{t}={GF}_{t}+{CF}_{t}+{IF}_{t}
\end{dmath}
% Equation 61
\begin{dmath}
{KF}_{t}=\left(1-{SF}_{t}\right)\, {IF}_{t}+\left(1-{{\delta}}\right)\, {KF}_{t-1}
\end{dmath}
% Equation 62
\begin{dmath}
{XF}_{t}=\frac{{IF}_{t}}{{IF}_{t-1}}
\end{dmath}
% Equation 63
\begin{dmath}
{SF}_{t}={{\phi_{X}}}\, \left({XF}_{t}-1\right)^{2}
\end{dmath}
% Equation 64
\begin{dmath}
{SF^{l}}_{t}=2\, {{\phi_{X}}}\, \left({XF}_{t}-1\right)
\end{dmath}
% Equation 65
\begin{dmath}
{TaxF}_{t}={GF}_{t}
\end{dmath}
% Equation 66
\begin{dmath}
{PF^{W}}_{t}=1-\frac{1}{{{\zeta}}}
\end{dmath}
% Equation 67
\begin{dmath}
{OUTGAP}_{t}=\frac{{YF}_{t}}{{Y}_{t}}
\end{dmath}
% Equation 68
\begin{dmath}
{\frac{\bar{KF}}{\bar{YF}}}_{t}=\frac{{KF}_{t}}{{YF}_{t}}
\end{dmath}
% Equation 69
\begin{dmath}
{\frac{\bar{IF}}{\bar{YF}}}_{t}=\frac{{IF}_{t}}{{YF}_{t}}
\end{dmath}
% Equation 70
\begin{dmath}
{\frac{\bar{CF}}{\bar{YF}}}_{t}=\frac{{CF}_{t}}{{YF}_{t}}
\end{dmath}
