% Equation 1
\begin{dmath}
{{\varrho}}=({{\varrho}})
\end{dmath}
% Equation 2
\begin{dmath}
{U}=\frac{\left(\left({C}-{C}\, {{\chi}}\right)^{1-{{\varrho}}}\, \left(1-{H}\right)^{{{\varrho}}}\right)^{1-{{\sigma_{C}}}}-1}{1-{{\sigma_{C}}}}
\end{dmath}
% Equation 3
\begin{dmath}
{UC}=\left(1-{{\varrho}}\right)\, \left({C}-{C}\, {{\chi}}\right)^{\left(1-{{\varrho}}\right)\, \left(1-{{\sigma_{C}}}\right)-1}\, \left(1-{H}\right)^{{{\varrho}}\, \left(1-{{\sigma_{C}}}\right)}
\end{dmath}
% Equation 4
\begin{dmath}
{UH}=\left(-{{\varrho}}\right)\, \left({C}-{C}\, {{\chi}}\right)^{\left(1-{{\varrho}}\right)\, \left(1-{{\sigma_{C}}}\right)}\, \left(1-{H}\right)^{{{\varrho}}\, \left(1-{{\sigma_{C}}}\right)-1}
\end{dmath}
% Equation 5
\begin{dmath}
{\lambda}={{\beta}}
\end{dmath}
% Equation 6
\begin{dmath}
{\lambda}\, {R}=1
\end{dmath}
% Equation 7
\begin{dmath}
{R}=\frac{{Rn}}{{\pi}}
\end{dmath}
% Equation 8
\begin{dmath}
{E(R)}=\frac{{Rn}}{{\pi}}
\end{dmath}
% Equation 9
\begin{dmath}
\frac{\left(-{UH}\right)}{{UC}}={W}
\end{dmath}
% Equation 10
\begin{dmath}
{\delta}={\delta}\, {{\xi}}\, {\tilde{\pi}}^{{{\zeta}}}+\left(1-{{\xi}}\right)\, \left(\frac{{J}}{{JJ}}\right)^{\left(-{{\zeta}}\right)}
\end{dmath}
% Equation 11
\begin{dmath}
{Y}=\frac{\left({H}\, {A}\right)^{{{\alpha}}}\, {K}^{1-{{\alpha}}}}{{\delta}}
\end{dmath}
% Equation 12
\begin{dmath}
{R^{K}}=\frac{\frac{{\delta}\, {Y}\, \left(1-{{\alpha}}\right)\, {P^{W}}}{{K}}+\left(1-{{\delta}}\right)\, {Q}}{{Q}}
\end{dmath}
% Equation 13
\begin{dmath}
{Q}\, \left(1-{S}-{X}\, {S^{l}}\right)+{S^{l}}\, {\lambda}\, {Q}\, {X}^{2}=1
\end{dmath}
% Equation 14
\begin{dmath}
{\lambda}\, {R^{K}}=1
\end{dmath}
% Equation 15
\begin{dmath}
\frac{{P^{W}}\, {\delta}\, {Y}\, {{\alpha}}}{{H}}={W}
\end{dmath}
% Equation 16
\begin{dmath}
{Y}={C}+{G}+{I}
\end{dmath}
% Equation 17
\begin{dmath}
{K}=\left(1-{S}\right)\, {I}+{K}\, \left(1-{{\delta}}\right)
\end{dmath}
% Equation 18
\begin{dmath}
{X}=1
\end{dmath}
% Equation 19
\begin{dmath}
{S}={{\phi_{X}}}\, \left({X}-1\right)^{2}
\end{dmath}
% Equation 20
\begin{dmath}
{S^{l}}=\left({X}-1\right)\, 2\, {{\phi_{X}}}
\end{dmath}
% Equation 21
\begin{dmath}
{G}={Tax}
\end{dmath}
% Equation 22
\begin{dmath}
{JJ}-{{\beta}}\, {{\xi}}\, {\tilde{JJ}}={UC}\, {Y}
\end{dmath}
% Equation 23
\begin{dmath}
{J}-{{\beta}}\, {{\xi}}\, {\tilde{J}}={UC}\, {Y}\, \frac{1}{1-\frac{1}{{{\zeta}}}}\, {MC}\, {MS}
\end{dmath}
% Equation 24
\begin{dmath}
{\tilde{JJ}}={JJ}\, {\tilde{\pi}}^{{{\zeta}}-1}
\end{dmath}
% Equation 25
\begin{dmath}
{\tilde{J}}={\tilde{\pi}}^{{{\zeta}}}\, {J}
\end{dmath}
% Equation 26
\begin{dmath}
1={{\xi}}\, {\tilde{\pi}}^{{{\zeta}}-1}+\left(1-{{\xi}}\right)\, \left(\frac{{J}}{{JJ}}\right)^{1-{{\zeta}}}
\end{dmath}
% Equation 27
\begin{dmath}
{\tilde{\pi}}=\frac{{\pi}}{{\pi}^{{{\gamma^{p}}}}}
\end{dmath}
% Equation 28
\begin{dmath}
\log\left(\frac{{Rn}}{({Rn})}\right)=\log\left(\frac{{Rn}}{({Rn})}\right)\, {{\rho_{R}}}+\left(1-{{\rho_{R}}}\right)\, {\theta^{\pi}}\, \log\left(\frac{{\pi}}{({\pi})}\right)+\left(1-{{\rho_{R}}}\right)\, {\theta^{y}}\, \log\left(\frac{{Y}}{({Y})}\right)+{{\sigma_{M}}}\, {{\epsilon^{M}}}
\end{dmath}
% Equation 29
\begin{dmath}
{MC}={P^{W}}
\end{dmath}
% Equation 30
\begin{dmath}
\log\left({A}\right)-\log\left(({A})\right)=\left(\log\left({A}\right)-\log\left(({A})\right)\right)\, {{\rho_{A}}}+{{\sigma_{A}}}\, {{\epsilon^{A}}}
\end{dmath}
% Equation 31
\begin{dmath}
\log\left({G}\right)-\log\left(({G})\right)=\left(\log\left({G}\right)-\log\left(({G})\right)\right)\, {{\rho_{G}}}+{{\sigma_{G}}}\, {{\epsilon^{G}}}
\end{dmath}
% Equation 32
\begin{dmath}
\log\left({GF}\right)-\log\left(({GF})\right)={{\sigma_{G}}}\, {{\epsilon^{G}}}+{{\rho_{G}}}\, \left(\log\left({GF}\right)-\log\left(({GF})\right)\right)
\end{dmath}
% Equation 33
\begin{dmath}
\log\left({MS}\right)-\log\left(({MS})\right)=\left(\log\left({MS}\right)-\log\left(({MS})\right)\right)\, {{\rho_{MS}}}+{{\sigma_{MS}}}\, {{\epsilon^{MS}}}
\end{dmath}
% Equation 34
\begin{dmath}
{yy}=\frac{{Y}}{({Y})}
\end{dmath}
% Equation 35
\begin{dmath}
{kk}=\frac{{K}}{({K})}
\end{dmath}
% Equation 36
\begin{dmath}
{ii}=\frac{{I}}{({I})}
\end{dmath}
% Equation 37
\begin{dmath}
{cc}=\frac{{C}}{({C})}
\end{dmath}
% Equation 38
\begin{dmath}
{ww}=\frac{{W}}{({W})}
\end{dmath}
% Equation 39
\begin{dmath}
{hh}=\frac{{H}}{({H})}
\end{dmath}
% Equation 40
\begin{dmath}
{qq}=\frac{{Q}}{({Q})}
\end{dmath}
% Equation 41
\begin{dmath}
{RR}=\frac{{R}}{({R})}
\end{dmath}
% Equation 42
\begin{dmath}
{E(RR)}=\frac{{E(R)}}{({E(R)})}
\end{dmath}
% Equation 43
\begin{dmath}
{RRn}=\frac{{Rn}}{({Rn})}
\end{dmath}
% Equation 44
\begin{dmath}
{\pi\pi}=\frac{{\pi}}{({\pi})}
\end{dmath}
% Equation 45
\begin{dmath}
{Ogapogap}=\frac{{OUTGAP}}{({OUTGAP})}
\end{dmath}
% Equation 46
\begin{dmath}
{\frac{\bar{K}}{\bar{YW}}}=\frac{{K}}{{Y}}
\end{dmath}
% Equation 47
\begin{dmath}
{\frac{\bar{I}}{\bar{Y}}}=\frac{{I}}{{Y}}
\end{dmath}
% Equation 48
\begin{dmath}
{\frac{\bar{C}}{\bar{Y}}}=\frac{{C}}{{Y}}
\end{dmath}
% Equation 49
\begin{dmath}
{UF}=\frac{\left(\left({CF}-{{\chi}}\, {CF}\right)^{1-{{\varrho}}}\, \left(1-{HF}\right)^{{{\varrho}}}\right)^{1-{{\sigma_{C}}}}-1}{1-{{\sigma_{C}}}}
\end{dmath}
% Equation 50
\begin{dmath}
{UCF}=\left(1-{{\varrho}}\right)\, \left({CF}-{{\chi}}\, {CF}\right)^{\left(1-{{\varrho}}\right)\, \left(1-{{\sigma_{C}}}\right)-1}\, \left(1-{HF}\right)^{{{\varrho}}\, \left(1-{{\sigma_{C}}}\right)}
\end{dmath}
% Equation 51
\begin{dmath}
{ULF}=\left(-{{\varrho}}\right)\, \left({CF}-{{\chi}}\, {CF}\right)^{\left(1-{{\varrho}}\right)\, \left(1-{{\sigma_{C}}}\right)}\, \left(1-{HF}\right)^{{{\varrho}}\, \left(1-{{\sigma_{C}}}\right)-1}
\end{dmath}
% Equation 52
\begin{dmath}
{\lambda}={{\beta}}
\end{dmath}
% Equation 53
\begin{dmath}
{\lambda}\, {RF}=1
\end{dmath}
% Equation 54
\begin{dmath}
\frac{\left(-{ULF}\right)}{{UCF}}={WF}
\end{dmath}
% Equation 55
\begin{dmath}
{YF}=\left({A}\, {HF}\right)^{{{\alpha}}}\, {KF}^{1-{{\alpha}}}
\end{dmath}
% Equation 56
\begin{dmath}
{RFk}=\frac{\frac{{YF}\, \left(1-{{\alpha}}\right)\, {PF^{W}}}{{KF}}+\left(1-{{\delta}}\right)\, {QF}}{{QF}}
\end{dmath}
% Equation 57
\begin{dmath}
{QF}\, \left(1-{SF}-{XF}\, {SF^{l}}\right)+{SF^{l}}\, {\lambda}\, {QF}\, {XF}^{2}=1
\end{dmath}
% Equation 58
\begin{dmath}
{\lambda}\, {RFk}=1
\end{dmath}
% Equation 59
\begin{dmath}
\frac{{PF^{W}}\, {{\alpha}}\, {YF}}{{HF}}={WF}
\end{dmath}
% Equation 60
\begin{dmath}
{YF}={GF}+{CF}+{IF}
\end{dmath}
% Equation 61
\begin{dmath}
{KF}=\left(1-{SF}\right)\, {IF}+\left(1-{{\delta}}\right)\, {KF}
\end{dmath}
% Equation 62
\begin{dmath}
{XF}=1
\end{dmath}
% Equation 63
\begin{dmath}
{SF}={{\phi_{X}}}\, \left({XF}-1\right)^{2}
\end{dmath}
% Equation 64
\begin{dmath}
{SF^{l}}=2\, {{\phi_{X}}}\, \left({XF}-1\right)
\end{dmath}
% Equation 65
\begin{dmath}
{TaxF}={GF}
\end{dmath}
% Equation 66
\begin{dmath}
{PF^{W}}=1-\frac{1}{{{\zeta}}}
\end{dmath}
% Equation 67
\begin{dmath}
{OUTGAP}=\frac{{YF}}{{Y}}
\end{dmath}
% Equation 68
\begin{dmath}
{\frac{\bar{KF}}{\bar{YF}}}=\frac{{KF}}{{YF}}
\end{dmath}
% Equation 69
\begin{dmath}
{\frac{\bar{IF}}{\bar{YF}}}=\frac{{IF}}{{YF}}
\end{dmath}
% Equation 70
\begin{dmath}
{\frac{\bar{CF}}{\bar{YF}}}=\frac{{CF}}{{YF}}
\end{dmath}
