% Equation 1
\begin{dmath}
{UCF}_{t}=\left(\left(1-{{\varrho}}\right)\, \left(1-{{\sigma_{C}}}\right)-1\right)\, \left(\frac{{CF}_{t}}{1-{{\chi}}}-\frac{{{\chi}}}{1-{{\chi}}}\, {CF}_{t-1}\right)+{{\varrho}}\, \left({{\sigma_{C}}}-1\right)\, \frac{{{\bar{H}}}}{1-{{\bar{H}}}}\, {HF}_{t}
\end{dmath}
% Equation 2
\begin{dmath}
{UCF}_{t+1}={UCF}_{t}-{RF}_{t}
\end{dmath}
% Equation 3
\begin{dmath}
{ULF}_{t}=\left(-{UCF}_{t}\right)-\left(\frac{{CF}_{t}}{1-{{\chi}}}-\frac{{{\chi}}}{1-{{\chi}}}\, {CF}_{t-1}\right)-\frac{{{\bar{H}}}}{1-{{\bar{H}}}}\, {HF}_{t}
\end{dmath}
% Equation 4
\begin{dmath}
{WF}_{t}=\left(-{ULF}_{t}\right)-{UCF}_{t}
\end{dmath}
% Equation 5
\begin{dmath}
{YF}_{t}={{\alpha}}\, \left({HF}_{t}+{A}_{t}\right)+\left(1-{{\alpha}}\right)\, {KF}_{t-1}
\end{dmath}
% Equation 6
\begin{dmath}
{WF}_{t}={YF}_{t}-{HF}_{t}
\end{dmath}
% Equation 7
\begin{dmath}
{YF}_{t}={CF}_{t}\, {{cyf}}+{{iyf}}\, {IF}_{t}+{{gy}}\, {GF}_{t}
\end{dmath}
% Equation 8
\begin{dmath}
{KF}_{t}={IF}_{t}\, {{\delta}}+{KF}_{t-1}\, \left(1-{{\delta}}\right)
\end{dmath}
% Equation 9
\begin{dmath}
{XF}_{t}=\frac{{{\delta}}+{{\bar{RF}}}-1}{{{\bar{RF}}}}\, \left({YF}_{t}-{KF}_{t-1}\right)+\frac{1-{{\delta}}}{{{\bar{RF}}}}\, {QF}_{t}
\end{dmath}
% Equation 10
\begin{dmath}
{RF}_{t}={XF}_{t+1}-{QF}_{t}
\end{dmath}
% Equation 11
\begin{dmath}
{IF}_{t}\, \left(1+\frac{1}{{{\bar{RF}}}}\right)=\frac{1}{{{\bar{RF}}}}\, {IF}_{t+1}+{IF}_{t-1}+{QF}_{t}\, \frac{1}{2\, {{\phi_{X}}}}
\end{dmath}
% Equation 12
\begin{dmath}
{GF}_{t}={HF}_{t}+{WF}_{t}+{TaxF}_{t}
\end{dmath}
% Equation 13
\begin{dmath}
{GF}_{t}={{\rho_{G}}}\, {GF}_{t-1}+{{\epsilon^{G}}}_{t}
\end{dmath}
% Equation 14
\begin{dmath}
{UC}_{t}=\left(\left(1-{{\varrho}}\right)\, \left(1-{{\sigma_{C}}}\right)-1\right)\, \left(\frac{{C}_{t}}{1-{{\chi}}}-\frac{{{\chi}}}{1-{{\chi}}}\, {C}_{t-1}\right)+{{\varrho}}\, \left({{\sigma_{C}}}-1\right)\, \frac{{{\bar{H}}}}{1-{{\bar{H}}}}\, {H}_{t}
\end{dmath}
% Equation 15
\begin{dmath}
{UC}_{t+1}={UC}_{t}-{R}_{t+1}
\end{dmath}
% Equation 16
\begin{dmath}
{UH}_{t}=\left(-{UC}_{t}\right)-\left(\frac{{C}_{t}}{1-{{\chi}}}-\frac{{{\chi}}}{1-{{\chi}}}\, {C}_{t-1}\right)-\frac{{{\bar{H}}}}{1-{{\bar{H}}}}\, {H}_{t}
\end{dmath}
% Equation 17
\begin{dmath}
{W}_{t}=\left(-{UH}_{t}\right)-{UC}_{t}
\end{dmath}
% Equation 18
\begin{dmath}
{Y}_{t}={{\alpha}}\, \left({A}_{t}+{H}_{t}\right)+\left(1-{{\alpha}}\right)\, {K}_{t-1}
\end{dmath}
% Equation 19
\begin{dmath}
{MC}_{t}={H}_{t}+{W}_{t}-{Y}_{t}
\end{dmath}
% Equation 20
\begin{dmath}
{Y}_{t}={C}_{t}\, {{cy}}+{{iy}}\, {I}_{t}+{{gy}}\, {G}_{t}
\end{dmath}
% Equation 21
\begin{dmath}
{K}_{t}={{\delta}}\, {I}_{t}+\left(1-{{\delta}}\right)\, {K}_{t-1}
\end{dmath}
% Equation 22
\begin{dmath}
{X}_{t}=\frac{{{\delta}}+{{\bar{R}}}-1}{{{\bar{R}}}}\, \left({Y}_{t}+{MC}_{t}-{K}_{t-1}\right)+\frac{1-{{\delta}}}{{{\bar{R}}}}\, {Q}_{t}
\end{dmath}
% Equation 23
\begin{dmath}
{R}_{t+1}={X}_{t+1}-{Q}_{t}
\end{dmath}
% Equation 24
\begin{dmath}
{I}_{t}\, \left(1+\frac{1}{{{\bar{R}}}}\right)=\frac{1}{{{\bar{R}}}}\, {I}_{t+1}+{I}_{t-1}+\frac{1}{2\, {{\phi_{X}}}}\, {Q}_{t}
\end{dmath}
% Equation 25
\begin{dmath}
{G}_{t}={H}_{t}+{W}_{t}+{Tax}_{t}
\end{dmath}
% Equation 26
\begin{dmath}
{Pi}_{t}=\frac{{{\beta}}}{1+{{\beta}}\, {{\gamma^{p}}}}\, {Pi}_{t+1}+\frac{{{\gamma^{p}}}}{1+{{\beta}}\, {{\gamma^{p}}}}\, {Pi}_{t-1}+\frac{\left(1-{{\beta}}\, {{\xi}}\right)\, \left(1-{{\xi}}\right)}{\left(1+{{\beta}}\, {{\gamma^{p}}}\right)\, {{\xi}}}\, \left({MC}_{t}+{MS}_{t}\right)
\end{dmath}
% Equation 27
\begin{dmath}
{Rn}_{t}={{\rho_{R}}}\, {Rn}_{t-1}+{Pi}_{t}\, \left(1-{{\rho_{R}}}\right)\, {\theta^{\pi}}+{Y}_{t}\, \left(1-{{\rho_{R}}}\right)\, {\theta^{y}}+{{\epsilon^{M}}}_{t}
\end{dmath}
% Equation 28
\begin{dmath}
{R}_{t}={Rn}_{t-1}-{Pi}_{t}
\end{dmath}
% Equation 29
\begin{dmath}
{E(R)}_{t}={Rn}_{t}-{Pi}_{t+1}
\end{dmath}
% Equation 30
\begin{dmath}
{A}_{t}={{\rho_{A}}}\, {A}_{t-1}+{{\epsilon^{A}}}_{t}
\end{dmath}
% Equation 31
\begin{dmath}
{G}_{t}={{\epsilon^{G}}}_{t}+{{\rho_{G}}}\, {G}_{t-1}
\end{dmath}
% Equation 32
\begin{dmath}
{MS}_{t}={{\rho_{MS}}}\, {MS}_{t-1}+{{\epsilon^{MS}}}_{t}
\end{dmath}
