% Equation 1
\begin{dmath}
{U}_{t}=\frac{\left({C}_{t}^{1-{{\varrho}}}\, \left(1-{H}_{t}\right)^{{{\varrho}}}\right)^{1-{{\sigma_{C}}}}-1}{1-{{\sigma_{C}}}}
\end{dmath}
% Equation 2
\begin{dmath}
{U_C}_{t}=\left(1-{{\varrho}}\right)\, {C}_{t}^{\left(1-{{\varrho}}\right)\, \left(1-{{\sigma_{C}}}\right)-1}\, \left(1-{H}_{t}\right)^{{{\varrho}}\, \left(1-{{\sigma_{C}}}\right)}
\end{dmath}
% Equation 3
\begin{dmath}
{U_H}_{t}=\left(-{{\varrho}}\right)\, {C}_{t}^{\left(1-{{\varrho}}\right)\, \left(1-{{\sigma_{C}}}\right)}\, \left(1-{H}_{t}\right)^{{{\varrho}}\, \left(1-{{\sigma_{C}}}\right)-1}
\end{dmath}
% Equation 4
\begin{dmath}
{\Lambda}_{t}\, {R}_{t}=1
\end{dmath}
% Equation 5
\begin{dmath}
\frac{\left(-{U_H}_{t}\right)}{{U_C}_{t}}={W}_{t}
\end{dmath}
% Equation 6
\begin{dmath}
{Y}_{t}=\left({H}_{t}\, {A}_{t}\right)^{{{\alpha}}}\, {K}_{t-1}^{1-{{\alpha}}}
\end{dmath}
% Equation 7
\begin{dmath}
\frac{{Y}_{t}\, {{\alpha}}}{{H}_{t}}={W}_{t}
\end{dmath}
% Equation 8
\begin{dmath}
{Y}_{t}={C}_{t}+{G}_{t}+{I}_{t}
\end{dmath}
% Equation 9
\begin{dmath}
{K}_{t}={I}_{t}\, \left(1-{{\phi^X}}\, \left(\frac{{I}_{t}}{{I}_{t-1}}-1\right)^{2}\right)+{K}_{t-1}\, \left(1-{{\delta}}\right)
\end{dmath}
% Equation 10
\begin{dmath}
{\Lambda}_{t}=\frac{{{\beta}}\, {U_C}_{t+1}}{{U_C}_{t}}
\end{dmath}
% Equation 11
\begin{dmath}
1={q}_{t}\, \left(1-{{\phi^X}}\, \left(\frac{{I}_{t}}{{I}_{t-1}}-1\right)^{2}-\frac{{I}_{t}}{{I}_{t-1}}\, \left(\frac{{I}_{t}}{{I}_{t-1}}-1\right)\, 2\, {{\phi^X}}\right)+{{\phi^X}}\, 2\, {\Lambda}_{t}\, {q}_{t+1}\, \left(\frac{{I}_{t+1}}{{I}_{t}}-1\right)\, \left(\frac{{I}_{t+1}}{{I}_{t}}\right)^{2}
\end{dmath}
% Equation 12
\begin{dmath}
{r^{K}}_{t}=\frac{{Y}_{t}\, \left(1-{{\alpha}}\right)}{{K}_{t-1}}
\end{dmath}
% Equation 13
\begin{dmath}
{R^{K}}_{t}=\frac{{r^{K}}_{t+1}+\left(1-{{\delta}}\right)\, {q}_{t+1}}{{q}_{t}}
\end{dmath}
% Equation 14
\begin{dmath}
{\Lambda}_{t}\, {R^{K}}_{t}=1
\end{dmath}
% Equation 15
\begin{dmath}
{G}_{t}={T}_{t}
\end{dmath}
% Equation 16
\begin{dmath}
\log\left({A}_{t}\right)-\log\left((\bar{A})\right)={{\rho_{A}}}\, \left(\log\left({A}_{t-1}\right)-\log\left((\bar{A})\right)\right)+{{\sigma}}\, {{\epsilon^{A}}}_{t}
\end{dmath}
% Equation 17
\begin{dmath}
\log\left({G}_{t}\right)-\log\left((\bar{G})\right)={{\rho_{G}}}\, \left(\log\left({G}_{t-1}\right)-\log\left((\bar{G})\right)\right)+{{\sigma}}\, {{\epsilon^{G}}}_{t}
\end{dmath}
% Equation 18
\begin{dmath}
{YY}_{t}=\frac{{Y}_{t}}{(\bar{Y})}
\end{dmath}
% Equation 19
\begin{dmath}
{KK}_{t}=\frac{{K}_{t}}{(\bar{K})}
\end{dmath}
% Equation 20
\begin{dmath}
{II}_{t}=\frac{{I}_{t}}{(\bar{I})}
\end{dmath}
% Equation 21
\begin{dmath}
{CC}_{t}=\frac{{C}_{t}}{(\bar{C})}
\end{dmath}
% Equation 22
\begin{dmath}
{WW}_{t}=\frac{{W}_{t}}{(\bar{W})}
\end{dmath}
% Equation 23
\begin{dmath}
{HH}_{t}=\frac{{H}_{t}}{(\bar{H})}
\end{dmath}
% Equation 24
\begin{dmath}
{RR}_{t}=\frac{{R}_{t}}{(\bar{R})}
\end{dmath}
% Equation 25
\begin{dmath}
{\frac{\bar{K}}{\bar{Y}}}_{t}=\frac{{K}_{t}}{{Y}_{t}}
\end{dmath}
% Equation 26
\begin{dmath}
{\frac{\bar{I}}{\bar{Y}}}_{t}=\frac{{I}_{t}}{{Y}_{t}}
\end{dmath}
% Equation 27
\begin{dmath}
{\frac{\bar{C}}{\bar{Y}}}_{t}=\frac{{C}_{t}}{{Y}_{t}}
\end{dmath}
