% Equation 1
\begin{dmath}
{U}=\frac{\left({C}^{1-{{\varrho}}}\, \left(1-{H}\right)^{{{\varrho}}}\right)^{1-{{\sigma_{C}}}}-1}{1-{{\sigma_{C}}}}
\end{dmath}
% Equation 2
\begin{dmath}
{U_C}=\left(1-{{\varrho}}\right)\, {C}^{\left(1-{{\varrho}}\right)\, \left(1-{{\sigma_{C}}}\right)-1}\, \left(1-{H}\right)^{{{\varrho}}\, \left(1-{{\sigma_{C}}}\right)}
\end{dmath}
% Equation 3
\begin{dmath}
{U_H}=\left(-{{\varrho}}\right)\, {C}^{\left(1-{{\varrho}}\right)\, \left(1-{{\sigma_{C}}}\right)}\, \left(1-{H}\right)^{{{\varrho}}\, \left(1-{{\sigma_{C}}}\right)-1}
\end{dmath}
% Equation 4
\begin{dmath}
{\Lambda}\, {R}=1
\end{dmath}
% Equation 5
\begin{dmath}
\frac{\left(-{U_H}\right)}{{U_C}}={W}
\end{dmath}
% Equation 6
\begin{dmath}
{Y}=\left({H}\, {A}\right)^{{{\alpha}}}\, {K}^{1-{{\alpha}}}
\end{dmath}
% Equation 7
\begin{dmath}
\frac{{Y}\, {{\alpha}}}{{H}}={W}
\end{dmath}
% Equation 8
\begin{dmath}
{Y}={C}+{G}+{I}
\end{dmath}
% Equation 9
\begin{dmath}
{K}={I}+{K}\, \left(1-{{\delta}}\right)
\end{dmath}
% Equation 10
\begin{dmath}
{\Lambda}={{\beta}}
\end{dmath}
% Equation 11
\begin{dmath}
1={q}
\end{dmath}
% Equation 12
\begin{dmath}
{r^{K}}=\frac{{Y}\, \left(1-{{\alpha}}\right)}{{K}}
\end{dmath}
% Equation 13
\begin{dmath}
{R^{K}}=\frac{{r^{K}}+\left(1-{{\delta}}\right)\, {q}}{{q}}
\end{dmath}
% Equation 14
\begin{dmath}
{\Lambda}\, {R^{K}}=1
\end{dmath}
% Equation 15
\begin{dmath}
{G}={T}
\end{dmath}
% Equation 16
\begin{dmath}
\log\left({A}\right)-\log\left(({A})\right)=\left(\log\left({A}\right)-\log\left(({A})\right)\right)\, {{\rho_{A}}}+{{\sigma}}\, {{\epsilon^{A}}}
\end{dmath}
% Equation 17
\begin{dmath}
\log\left({G}\right)-\log\left(({G})\right)=\left(\log\left({G}\right)-\log\left(({G})\right)\right)\, {{\rho_{G}}}+{{\sigma}}\, {{\epsilon^{G}}}
\end{dmath}
% Equation 18
\begin{dmath}
{YY}=\frac{{Y}}{({Y})}
\end{dmath}
% Equation 19
\begin{dmath}
{KK}=\frac{{K}}{({K})}
\end{dmath}
% Equation 20
\begin{dmath}
{II}=\frac{{I}}{({I})}
\end{dmath}
% Equation 21
\begin{dmath}
{CC}=\frac{{C}}{({C})}
\end{dmath}
% Equation 22
\begin{dmath}
{WW}=\frac{{W}}{({W})}
\end{dmath}
% Equation 23
\begin{dmath}
{HH}=\frac{{H}}{({H})}
\end{dmath}
% Equation 24
\begin{dmath}
{RR}=\frac{{R}}{({R})}
\end{dmath}
% Equation 25
\begin{dmath}
{\frac{\bar{K}}{\bar{Y}}}=\frac{{K}}{{Y}}
\end{dmath}
% Equation 26
\begin{dmath}
{\frac{\bar{I}}{\bar{Y}}}=\frac{{I}}{{Y}}
\end{dmath}
% Equation 27
\begin{dmath}
{\frac{\bar{C}}{\bar{Y}}}=\frac{{C}}{{Y}}
\end{dmath}
