% Equation 1
\begin{dmath}
{U^{C}}=\left(\left(1-{{\varrho}}\right)\, \left(1-{{\sigma_{C}}}\right)-1\right)\, {C}+{{\varrho}}\, \left({{\sigma_{C}}}-1\right)\, \frac{{\bar{H}}}{1-{\bar{H}}}\, {H}
\end{dmath}
% Equation 2
\begin{dmath}
{U^{C}}={U^{C}}-{R}
\end{dmath}
% Equation 3
\begin{dmath}
{U^{L}}={U^{C}}+{C}+\frac{{\bar{H}}}{1-{\bar{H}}}\, {H}
\end{dmath}
% Equation 4
\begin{dmath}
{W}={U^{L}}-{U^{C}}
\end{dmath}
% Equation 5
\begin{dmath}
{Y}={{\alpha}}\, \left({H}+{A}\right)+\left(1-{{\alpha}}\right)\, {K}
\end{dmath}
% Equation 6
\begin{dmath}
{Y}-{K}={R}\, \frac{{\bar{R}}}{{\bar{R}}-1+{{\delta}}}
\end{dmath}
% Equation 7
\begin{dmath}
{W}={Y}-{H}
\end{dmath}
% Equation 8
\begin{dmath}
{Y}={C}\, {\frac{\bar{C}}{\bar{Y}}}+{\frac{\bar{I}}{\bar{Y}}}\, {I}+{\frac{\bar{G}}{\bar{Y}}}\, {G}
\end{dmath}
% Equation 9
\begin{dmath}
{K}={{\delta}}\, {I}+{K}\, \left(1-{{\delta}}\right)
\end{dmath}
% Equation 10
\begin{dmath}
{A}={A}\, {{\rho_{A}}}+{{\sigma}}\, {{\epsilon^{A}}}
\end{dmath}
% Equation 11
\begin{dmath}
{G}={G}\, {{\rho_{G}}}+{{\sigma}}\, {{\epsilon^{G}}}
\end{dmath}
