% Equation 1
\begin{dmath}
{U}=\frac{\left(\left({C}-{C}\, {{\chi}}\right)^{1-{{\varrho}}}\, \left(1-{H}\right)^{{{\varrho}}}\right)^{1-{{\sigma_{C}}}}-1}{1-{{\sigma_{C}}}}
\end{dmath}
% Equation 2
\begin{dmath}
{UC}=\left(1-{{\varrho}}\right)\, \left({C}-{C}\, {{\chi}}\right)^{\left(1-{{\varrho}}\right)\, \left(1-{{\sigma_{C}}}\right)-1}\, \left(1-{H}\right)^{{{\varrho}}\, \left(1-{{\sigma_{C}}}\right)}
\end{dmath}
% Equation 3
\begin{dmath}
{UH}=\left(-{{\varrho}}\right)\, \left({C}-{C}\, {{\chi}}\right)^{\left(1-{{\varrho}}\right)\, \left(1-{{\sigma_{C}}}\right)}\, \left(1-{H}\right)^{{{\varrho}}\, \left(1-{{\sigma_{C}}}\right)-1}
\end{dmath}
% Equation 4
\begin{dmath}
{UC}={UC}\, {{\beta}}\, {R}
\end{dmath}
% Equation 5
\begin{dmath}
\frac{\left(-{UH}\right)}{{UC}}={W}
\end{dmath}
% Equation 6
\begin{dmath}
{Y}=\left({H}\, {A}\right)^{{{\alpha}}}\, {K}^{1-{{\alpha}}}
\end{dmath}
% Equation 7
\begin{dmath}
\frac{{Y}\, {{\alpha}}}{{H}}={W}
\end{dmath}
% Equation 8
\begin{dmath}
{Y}={C}+{G}+{I}
\end{dmath}
% Equation 9
\begin{dmath}
{K}={I}\, \left(1-{{\phi^X}}\, \left({X}-1\right)^{2}\right)+{K}\, \left(1-{{\delta}}\right)
\end{dmath}
% Equation 10
\begin{dmath}
{X}=1
\end{dmath}
% Equation 11
\begin{dmath}
{\lambda}={{\beta}}
\end{dmath}
% Equation 12
\begin{dmath}
{Z1}={\lambda}\, \left({X}-1\right)\, 2\, {{\phi^X}}\, {X}^{2}\, {Q}
\end{dmath}
% Equation 13
\begin{dmath}
{Z1}+{Q}\, \left(1-{{\phi^X}}\, \left({X}-1\right)^{2}-\left({X}-1\right)\, {{\phi^X}}\, 2\, {X}\right)=1
\end{dmath}
% Equation 14
\begin{dmath}
{R^{K}}=\frac{\frac{{Y}\, \left(1-{{\alpha}}\right)}{{K}}+\left(1-{{\delta}}\right)\, {Q}}{{Q}}
\end{dmath}
% Equation 15
\begin{dmath}
{\lambda}\, {R^{K}}={R}\, {\lambda}
\end{dmath}
% Equation 16
\begin{dmath}
{G}={H}\, {W}\, {T}
\end{dmath}
% Equation 17
\begin{dmath}
\log\left({A}\right)-\log\left(({A})\right)=\left(\log\left({A}\right)-\log\left(({A})\right)\right)\, {{\rho_{A}}}+{{\sigma}}\, {{\epsilon^{A}}}
\end{dmath}
% Equation 18
\begin{dmath}
\log\left({G}\right)-\log\left(({G})\right)=\left(\log\left({G}\right)-\log\left(({G})\right)\right)\, {{\rho_{G}}}+{{\sigma}}\, {{\epsilon^{G}}}
\end{dmath}
% Equation 19
\begin{dmath}
{YY}=\frac{{Y}}{({Y})}
\end{dmath}
% Equation 20
\begin{dmath}
{KK}=\frac{{K}}{({K})}
\end{dmath}
% Equation 21
\begin{dmath}
{II}=\frac{{I}}{({I})}
\end{dmath}
% Equation 22
\begin{dmath}
{CC}=\frac{{C}}{({C})}
\end{dmath}
% Equation 23
\begin{dmath}
{WW}=\frac{{W}}{({W})}
\end{dmath}
% Equation 24
\begin{dmath}
{HH}=\frac{{H}}{({H})}
\end{dmath}
% Equation 25
\begin{dmath}
{RR}=\frac{{R}}{({R})}
\end{dmath}
% Equation 26
\begin{dmath}
{\frac{\bar{K}}{\bar{Y}}}=\frac{{K}}{{Y}}
\end{dmath}
% Equation 27
\begin{dmath}
{\frac{\bar{I}}{\bar{Y}}}=\frac{{I}}{{Y}}
\end{dmath}
% Equation 28
\begin{dmath}
{\frac{\bar{C}}{\bar{Y}}}=\frac{{C}}{{Y}}
\end{dmath}
