% Equation 1
\begin{dmath}
{U}_{t}=\frac{\left({C}_{t}^{1-{{\varrho}}}\, \left(1-{H}_{t}\right)^{{{\varrho}}}\right)^{1-{{\sigma_{C}}}}-1}{1-{{\sigma_{C}}}}
\end{dmath}
% Equation 2
\begin{dmath}
{UC}_{t}=\left(1-{{\varrho}}\right)\, {C}_{t}^{\left(1-{{\varrho}}\right)\, \left(1-{{\sigma_{C}}}\right)-1}\, \left(1-{H}_{t}\right)^{{{\varrho}}\, \left(1-{{\sigma_{C}}}\right)}
\end{dmath}
% Equation 3
\begin{dmath}
{UL}_{t}=\left(-{{\varrho}}\right)\, {C}_{t}^{\left(1-{{\varrho}}\right)\, \left(1-{{\sigma_{C}}}\right)}\, \left(1-{H}_{t}\right)^{{{\varrho}}\, \left(1-{{\sigma_{C}}}\right)-1}
\end{dmath}
% Equation 4
\begin{dmath}
{\lambda}_{t}=\frac{{{\beta}}\, {UC}_{t+1}}{{UC}_{t}}
\end{dmath}
% Equation 5
\begin{dmath}
{UC}_{t}={UC}_{t+1}\, {{\beta}}\, {R}_{t}
\end{dmath}
% Equation 6
\begin{dmath}
{\lambda}_{t}\, {R^{K}}_{t}=1
\end{dmath}
% Equation 7
\begin{dmath}
\frac{\left(-{UL}_{t}\right)}{{UC}_{t}}={W}_{t}
\end{dmath}
% Equation 8
\begin{dmath}
{Y}_{t}=\left({H}_{t}\, {A}_{t}\right)^{{{\alpha}}}\, {K}_{t-1}^{1-{{\alpha}}}
\end{dmath}
% Equation 9
\begin{dmath}
\frac{{Y}_{t}\, {{\alpha}}}{{H}_{t}}={W}_{t}
\end{dmath}
% Equation 10
\begin{dmath}
{R^{K}}_{t}=1+\frac{\left(1-{{\alpha}}\right)\, {Y}_{t+1}}{{K}_{t}}-{{\delta}}
\end{dmath}
% Equation 11
\begin{dmath}
{Y}_{t}={C}_{t}+{G}_{t}+{I}_{t}
\end{dmath}
% Equation 12
\begin{dmath}
{K}_{t}={I}_{t}+{K}_{t-1}\, \left(1-{{\delta}}\right)
\end{dmath}
% Equation 13
\begin{dmath}
\log\left({A}_{t}\right)-\log\left((\bar{A})\right)={{\rho_{A}}}\, \left(\log\left({A}_{t-1}\right)-\log\left((\bar{A})\right)\right)+{{\sigma}}\, {{\epsilon^{A}}}_{t}
\end{dmath}
% Equation 14
\begin{dmath}
\log\left({G}_{t}\right)-\log\left((\bar{G})\right)={{\rho_{G}}}\, \left(\log\left({G}_{t-1}\right)-\log\left((\bar{G})\right)\right)+{{\sigma}}\, {{\epsilon^{G}}}_{t}
\end{dmath}
% Equation 15
\begin{dmath}
{y}_{t}=\log\left(\frac{{Y}_{t}}{(\bar{Y})}\right)
\end{dmath}
% Equation 16
\begin{dmath}
{k}_{t}=\log\left(\frac{{K}_{t}}{(\bar{K})}\right)
\end{dmath}
% Equation 17
\begin{dmath}
{i}_{t}=\log\left(\frac{{I}_{t}}{(\bar{I})}\right)
\end{dmath}
% Equation 18
\begin{dmath}
{c}_{t}=\log\left(\frac{{C}_{t}}{(\bar{C})}\right)
\end{dmath}
% Equation 19
\begin{dmath}
{w}_{t}=\log\left(\frac{{W}_{t}}{(\bar{W})}\right)
\end{dmath}
% Equation 20
\begin{dmath}
{h}_{t}=\log\left(\frac{{H}_{t}}{(\bar{H})}\right)
\end{dmath}
% Equation 21
\begin{dmath}
{r}_{t}=\log\left(\frac{{R}_{t}}{(\bar{R})}\right)
\end{dmath}
% Equation 22
\begin{dmath}
{a}_{t}=\log\left(\frac{{A}_{t}}{(\bar{A})}\right)
\end{dmath}
% Equation 23
\begin{dmath}
{g}_{t}=\log\left(\frac{{G}_{t}}{(\bar{G})}\right)
\end{dmath}
% Equation 24
\begin{dmath}
{\frac{\bar{K}}{\bar{Y}}}_{t}=\frac{{K}_{t}}{{Y}_{t}}
\end{dmath}
% Equation 25
\begin{dmath}
{\frac{\bar{I}}{\bar{Y}}}_{t}=\frac{{I}_{t}}{{Y}_{t}}
\end{dmath}
% Equation 26
\begin{dmath}
{\frac{\bar{C}}{\bar{Y}}}_{t}=\frac{{C}_{t}}{{Y}_{t}}
\end{dmath}
