% Equation 1
\begin{dmath}
{U^{C}}_{t}=\left(\left(1-{{\varrho}}\right)\, \left(1-{{\sigma_{C}}}\right)-1\right)\, \frac{{C}_{t}-{{\chi}}\, {C}_{t-1}}{1-{{\chi}}}+{{\varrho}}\, \left({{\sigma_{C}}}-1\right)\, \frac{{\bar{H}}}{1-{\bar{H}}}\, {H}_{t}
\end{dmath}
% Equation 2
\begin{dmath}
{U^{C}}_{t+1}={U^{C}}_{t}-{R}_{t}
\end{dmath}
% Equation 3
\begin{dmath}
{U^{L}}_{t}={U^{C}}_{t}+{C}_{t}+\frac{{\bar{H}}}{1-{\bar{H}}}\, {H}_{t}
\end{dmath}
% Equation 4
\begin{dmath}
{W}_{t}={U^{L}}_{t}-{U^{C}}_{t}
\end{dmath}
% Equation 5
\begin{dmath}
{Y}_{t}={{\alpha}}\, \left({H}_{t}+{A}_{t}\right)+\left(1-{{\alpha}}\right)\, {K}_{t-1}
\end{dmath}
% Equation 6
\begin{dmath}
{Y}_{t+1}-{K}_{t}={R}_{t}\, \frac{{\bar{R}}}{{\bar{R}}-1+{{\delta}}}
\end{dmath}
% Equation 7
\begin{dmath}
{W}_{t}={Y}_{t}-{H}_{t}
\end{dmath}
% Equation 8
\begin{dmath}
{Y}_{t}={C}_{t}\, {\frac{\bar{C}}{\bar{Y}}}+{\frac{\bar{I}}{\bar{Y}}}\, {I}_{t}+{\frac{\bar{G}}{\bar{Y}}}\, {G}_{t}
\end{dmath}
% Equation 9
\begin{dmath}
{K}_{t}={{\delta}}\, {I}_{t}+{K}_{t-1}\, \left(1-{{\delta}}\right)
\end{dmath}
% Equation 10
\begin{dmath}
{A}_{t}={{\rho_{A}}}\, {A}_{t-1}+{{\sigma}}\, {{\epsilon^{A}}}_{t}
\end{dmath}
% Equation 11
\begin{dmath}
{G}_{t}={{\rho_{G}}}\, {G}_{t-1}+{{\sigma}}\, {{\epsilon^{G}}}_{t}
\end{dmath}
